vale/specs/crypto/Vale.SHA2.Wrapper.fst
@@ -1,0 +1,15 @@
+module Vale.SHA2.Wrapper
+
+open FStar.UInt32
+open Spec.Agile.Hash
+open Spec.SHA2
+friend Lib.IntTypes
+friend Spec.SHA2
+
+let sigma256_0_0 x = v (_sigma0 SHA2_256 (uint_to_t x))
+
+let sigma256_0_1 x = v (_sigma1 SHA2_256 (uint_to_t x))
+
+let sigma256_1_0 x = v (_Sigma0 SHA2_256 (uint_to_t x))
+
+let sigma256_1_1 x = v (_Sigma1 SHA2_256 (uint_to_t x))
